theories/metaprogramming/substitution.v
@@ -1,0 +1,190 @@
+Require Import String.
+Require Import qterm.
+Require Import lambdaFacts.
+Require Import lambdaSolve.
+Require Import FunctionalExtensionality.
+Require Import Coq.Logic.PropExtensionality.
+
+Module S.
+  Definition nil := <Nil>.
+  Definition cons := <fun ctx => fun lvl => fun ty => Cons ctx lvl ty>.
+
+  Definition zero := <fun env => proj2 env>.
+  Definition succ := <fun x => fun env => x (proj1 env)>.
+
+  Definition level (n : nat) : QTerm := const n.
+
+  Definition pi := <fun x => fun y => fun env => Pi (x env) (fun a => y (env , a))>.
+  Definition U : QTerm := <fun env => U>.
+  Definition Empty := <fun env => Empty>.
+  Definition Bool := <fun env => Bool>.
+  Definition Lift := <fun T => fun env => Lift (T env)>.
+
+  Definition var_to_term := <fun x => x>.
+  Definition lambda := <fun t => fun env => fun a => t (env , a)>.
+  Definition app := <fun t1 => fun t2 => fun env => (t1 env) (t2 env)>.
+  Definition true := <fun env => fun p => proj1 p>.
+  Definition false := <fun env => fun p => proj2 p>.
+  Definition ifexpr := <fun cond => fun t1 => fun t2 => fun env => (cond env) (t1 env, t2 env)>.
+
+  Definition weaken := <fun t => fun env => t (proj1 env)>.
+  Definition subLast := <fun t => fun toSub => fun env => t (env , toSub env)>.
+
+  (* Shallow substitutions *)
+  Definition idSub := <fun env => env>. (* : Sub ctx ctx *)
+  Definition weaken1Ren := <fun env => proj1 env>. (* : Sub ctx (ctx, T) *)
+  (* liftSub : Sub ctx1 ctx2 -> Sub (cons ctx1 lvl T) (cons ctx2 lvl (subTerm sub T)) *)
+  Definition liftSub := <fun sub => fun env => (sub (proj1 env), proj2 env)>.
+  (* subTerm : (sub : Sub ctx1 ctx2) -> Term ctx1 T -> Term ctx2 (subTerm sub T) *)
+  Definition subTerm := <fun sub => fun t => fun env => t (sub env)>.
+
+  Ltac unfold_all := unfold nil, cons, zero, succ, pi, U, Bool, Empty, var_to_term, lambda,
+      app, weaken, subLast, level, true, false, ifexpr, Lift,
+      idSub, weaken1Ren, liftSub, subTerm in *.
+End S.
+
+(* The deeper shallow embedding *)
+
+Inductive Var : QTerm -> nat -> QTerm -> QTerm -> Type :=
+| zero : forall {ctx T lvl}, Var <`S.cons `ctx {const lvl} `T> lvl <`S.weaken `T> S.zero
+| succ : forall {ctx A T s lvl1 lvl2}, Var ctx lvl1 A s
+                              -> Var <`S.cons `ctx `lvl2 `T> lvl1 <`S.weaken `A> <`S.succ `s>.
+
+Inductive Typed : (*context*) QTerm -> (*level*) nat -> (*Type*) QTerm -> (*Term*) QTerm -> Type :=
+| lambda : forall {ctx A B s lvl},
+    (*Typed ctx (S lvl) <`U(*{const lvl}*)> <`pi `A `B> ->*)
+    Typed <`S.cons `ctx {const lvl} `A> lvl B s -> Typed ctx lvl <`S.pi `A `B> <`S.lambda `s>
+(*
+| app : forall ctx A B s1 s2 lvl, Typed ctx lvl <`pi `A `B> s1 -> Typed ctx lvl A s2
+                                 -> Typed ctx lvl <`subLast `B `s2> <`app `s1 `s2>*)
+| var : forall ctx T t lvl, Var ctx lvl T t -> Typed ctx lvl T t
+| true : forall {ctx}, Typed ctx 0 S.Bool S.true
+| false : forall {ctx}, Typed ctx 0 S.Bool S.false
+(*
+| if : forall ctx T cond t1 t2 lvl,
+    Typed ctx lvl Bool cond ->
+    Typed ctx lvl <`subLast `T `true> t1 ->
+    Typed ctx lvl <`subLast `T `false> t2 ->
+    Typed ctx lvl <`subLast `T `cond> <`ifexpr `cond `t1 `t2>
+| Empty : forall ctx, Typed ctx 1 <`U(*{const 0}*)> Empty
+| Bool : forall ctx, Typed ctx 1 <`U(*{const 0}*)> Bool
+| pi : forall ctx A B lvl,
+    Typed ctx (S lvl) <`U(*{const lvl}*)> A
+    (* TODO: is S lvl correct below? *)
+    -> Typed <`cons `ctx {const lvl} `A> (S lvl) <`U(*{const lvl}*)> B -> Typed ctx (S lvl) <`U(*{const lvl}*)> <`pi `A `B>
+| U : forall ctx lvl, Typed ctx (S (S lvl)) <`U(*{const (S lvl)}*)> <`U(*{const lvl}*)>
+| Lift : forall ctx lvl T, Typed ctx (S lvl) <`U> T -> Typed ctx (S (S lvl)) <`U> <`Lift `T>
+| lift : forall ctx lvl T t, Typed ctx lvl T t -> Typed ctx (S lvl) <`Lift `T> t
+| lower : forall ctx lvl T t, Typed ctx (S lvl) <`Lift `T> t -> Typed ctx lvl T t
+*)
+.
+
+Ltac solve_no_unfold := repeat (lambda_solve ; repeat neutral_inj_case ;lambda_solve
+                  ; repeat fast_neutral_unequal_case). 
+
+Ltac solve_all := repeat (S.unfold_all ; lambda_solve ; (repeat neutral_inj_case ;lambda_solve)
+                          ; (repeat fast_neutral_unequal_case); (repeat simple_pattern_case();
+                          (repeat pair_pattern_case; subst); rewrite <- ?eta, <- ?SP)).
+
+
+Definition cast {ctx1 ctx2 lvl1 lvl2 ty1 ty2 tm1 tm2}
+           {_ : ctx1 = ctx2}
+           {_ : lvl1 = lvl2}
+           {_ : ty1 = ty2}
+           {_ : tm1 = tm2}
+           (prog : Typed ctx1 lvl1 ty1 tm1) : Typed ctx2 lvl2 ty2 tm2.
+  subst.
+  apply prog.
+Defined.
+
+Definition castVar {ctx1 ctx2 lvl1 lvl2 ty1 ty2 tm1 tm2}
+           {_ : ctx1 = ctx2}
+           {_ : lvl1 = lvl2}
+           {_ : ty1 = ty2}
+           {_ : tm1 = tm2}
+           (prog : Var ctx1 lvl1 ty1 tm1) : Var ctx2 lvl2 ty2 tm2.
+  subst.
+  apply prog.
+Defined.
+
+Axiom uip : forall T (t1 t2 : T) (p1 p2 : t1 = t2), p1 = p2.
+Theorem remove_cast
+        (ctx ty tm : QTerm)
+        (lvl : nat)
+        (pctx : ctx = ctx)
+        (plvl : lvl = lvl)
+        (pty : ty = ty)
+        (ptm : tm = tm)
+        (input : Typed ctx lvl ty tm)
+        : @cast _ _ _ _ _ _ _ _ pctx plvl pty ptm input = input.
+Proof.
+  rewrite (uip _ _ _ pctx eq_refl).
+  rewrite (uip _ _ _ plvl eq_refl).
+  rewrite (uip _ _ _ pty eq_refl).
+  rewrite (uip _ _ _ ptm eq_refl).
+  reflexivity.
+Qed.
+
+Definition Ren (sub ctx1 ctx2 : QTerm) : Type :=
+  forall {lvl T t}, Var ctx1 lvl T t -> Var ctx2 lvl <`S.subTerm `sub `T> <`S.subTerm `sub `t>.
+
+Definition idRen {ctx} : Ren S.idSub ctx ctx.
+  refine (fun lvl T t x => castVar x); solve_all.
+Defined.
+
+Compute (1 + ltac:(exact 2)).
+
+Axiom hole : forall {T}, T.
+(*Definition idRen {ctx} : Ren S.idSub ctx ctx := fun lvl T t x => x.*)
+Definition liftRen {ctx1 ctx2 lvl T sub} (ren : Ren sub ctx1 ctx2)
+  : Ren <`S.liftSub `sub> <`S.cons `ctx1 `lvl `T> <`S.cons `ctx1 `lvl (`S.subTerm `sub `T)>.
+intros lvl2 T2 t2 x.
+remember <`S.cons `ctx1 `lvl `T> as ctx in x.
+generalize dependent Heqctx.
+refine (match x with
+        | @zero _ _ n => fun _ => castVar (@zero ctx1 <`S.subTerm `sub `T> n)
+        | succ x' => _ (*castVar (succ (ren _ _ _ _))*)
+        end); intros; solve_all.
+refine (castVar (@zero ctx1 <`S.subTerm `sub `T> n)); solve_all.
+rewrite <- SP.
+
+(*
+I can potentially fix solve_all to work around metavariables in the goal.
+But, also I can prevent there from being metavariables in the first place by giving arguments
+to "zero".
+*)
+
+
+(* normalize nonterminates here. Why? *)
+
+Print solve_all.
+S.unfold_all.
+Set Printing Goal Names.
+Unshelve.
+
+(*
+It appears that in practice, the evars only show up in the goal, not the context.
+*)
+
+repeat rewrite beta.
+rewrite subst_lam.
+simpl.
+(* TODO: right here is the point where I need to figure out what is going on
+with existential variables. Try running the next two tactics. *)
+
+
+rewrite lift_lam.
+simpl.
+
+repeat
+   (try (rewrite lift_lam; simpl); try rewrite lift_app; try rewrite lift_pair; try rewrite lift_pi1;
+     try rewrite lift_pi2; try (rewrite lift_var; simpl)).
+
+
+(*
+1) when you run solve when there are term metavariables, it nonterminates because it just keeps
+   refining the metavaraibles with every rewrite.
+2) But why even are there term metavariables? The idea of cast is that it should be specifically
+   the equality proofs that are left for later. Everything else should be defined in the refine.
+   So what is causing these terms to be left unspecified?
+*)
