theories/metaprogramming/test2.v
@@ -1,0 +1,168 @@
+
+Require Import String.
+Require Import qterm.
+Require Import lambdaFacts.
+Require Import lambdaSolve.
+Require Import FunctionalExtensionality.
+Require Import Coq.Logic.PropExtensionality.
+
+Definition nil := <Nil>.
+Definition cons := <fun ctx => fun lvl => fun ty => Cons ctx lvl ty>.
+
+Definition zero := <fun env => proj2 env>.
+Definition succ := <fun x => fun env => x (proj1 env)>.
+
+Definition level (n : nat) : QTerm := const n.
+(* Should I have an explicit type level on the pis? *)
+Definition pi := <fun x => fun y => fun env => Pi (x env) (fun a => y (env , a))>.
+Definition U : QTerm := <(*fun lvl => *)fun env => U (*lvl*)>.
+Definition Empty := <fun env => Empty>.
+Definition Bool := <fun env => Bool>.
+Definition Lift := <fun T => fun env => Lift (T env)>.
+
+Definition var_to_term := <fun x => x>.
+Definition lambda := <fun t => fun env => fun a => t (env , a)>.
+Definition app := <fun t1 => fun t2 => fun env => (t1 env) (t2 env)>.
+Definition true := <fun env => fun p => proj1 p>.
+Definition false := <fun env => fun p => proj2 p>.
+Definition ifexpr := <fun cond => fun t1 => fun t2 => fun env => (cond env) (t1 env, t2 env)>.
+
+Definition weaken := <fun t => fun env => t (proj1 env)>.
+Definition subLast := <fun t => fun toSub => fun env => t (env , toSub env)>.
+
+Ltac unfold_all := unfold nil, cons, zero, succ, pi, U, Bool, Empty, var_to_term, lambda,
+    app, weaken, subLast, level, true, false, ifexpr, Lift in *.
+
+(* The deeper shallow embedding *)
+
+Inductive VarTyped : QTerm -> nat -> QTerm -> QTerm -> Prop :=
+| ty_zero : forall ctx T lvl, VarTyped <`cons `ctx {const lvl} `T> lvl <`weaken `T> zero
+| ty_succ : forall ctx A T s lvl1 lvl2, VarTyped ctx lvl1 A s
+                              -> VarTyped <`cons `ctx `lvl2 `T> lvl1 <`weaken `A> <`succ `s>.
+
+Inductive Typed : (*context*) QTerm -> (*level*) nat -> (*Type*) QTerm -> (*Term*) QTerm -> Type :=
+| ty_lambda : forall {ctx A B s lvl},
+    (*Typed ctx (S lvl) <`U(*{const lvl}*)> <`pi `A `B> ->*)
+    Typed <`cons `ctx {const lvl} `A> lvl B s -> Typed ctx lvl <`pi `A `B> <`lambda `s>
+(*
+| ty_app : forall ctx A B s1 s2 lvl, Typed ctx lvl <`pi `A `B> s1 -> Typed ctx lvl A s2
+                                 -> Typed ctx lvl <`subLast `B `s2> <`app `s1 `s2>
+| ty_var : forall ctx T t lvl, VarTyped ctx lvl T t -> Typed ctx lvl T t
+*)
+| ty_true : forall {ctx}, Typed ctx 0 Bool true
+| ty_false : forall {ctx}, Typed ctx 0 Bool false
+(*
+| ty_if : forall ctx T cond t1 t2 lvl,
+    Typed ctx lvl Bool cond ->
+    Typed ctx lvl <`subLast `T `true> t1 ->
+    Typed ctx lvl <`subLast `T `false> t2 ->
+    Typed ctx lvl <`subLast `T `cond> <`ifexpr `cond `t1 `t2>
+| ty_Empty : forall ctx, Typed ctx 1 <`U(*{const 0}*)> Empty
+| ty_Bool : forall ctx, Typed ctx 1 <`U(*{const 0}*)> Bool
+| ty_pi : forall ctx A B lvl,
+    Typed ctx (S lvl) <`U(*{const lvl}*)> A
+    (* TODO: is S lvl correct below? *)
+    -> Typed <`cons `ctx {const lvl} `A> (S lvl) <`U(*{const lvl}*)> B -> Typed ctx (S lvl) <`U(*{const lvl}*)> <`pi `A `B>
+| ty_U : forall ctx lvl, Typed ctx (S (S lvl)) <`U(*{const (S lvl)}*)> <`U(*{const lvl}*)>
+| ty_Lift : forall ctx lvl T, Typed ctx (S lvl) <`U> T -> Typed ctx (S (S lvl)) <`U> <`Lift `T>
+| ty_lift : forall ctx lvl T t, Typed ctx lvl T t -> Typed ctx (S lvl) <`Lift `T> t
+| ty_lower : forall ctx lvl T t, Typed ctx (S lvl) <`Lift `T> t -> Typed ctx lvl T t
+*)
+.
+
+Ltac solve_no_unfold := repeat (lambda_solve ; repeat neutral_inj_case ;lambda_solve
+                  ; repeat fast_neutral_unequal_case). 
+
+Ltac solve_all := repeat (unfold_all ; lambda_solve ; repeat neutral_inj_case ;lambda_solve
+                          ; repeat fast_neutral_unequal_case; repeat simple_pattern_case;
+                          repeat pair_pattern_case; subst).
+
+
+Definition cast {ctx1 ctx2 lvl1 lvl2 ty1 ty2 tm1 tm2}
+           {_ : ctx1 = ctx2}
+           {_ : lvl1 = lvl2}
+           {_ : ty1 = ty2}
+           {_ : tm1 = tm2}
+           (prog : Typed ctx1 lvl1 ty1 tm1) : Typed ctx2 lvl2 ty2 tm2.
+  subst.
+  apply prog.
+Defined.
+
+Definition match_on_id {ctx T t: QTerm} {lvl} (prog : Typed ctx lvl T t)
+  :
+  ctx = nil
+  -> lvl = 0
+  -> T = <`pi `Bool `Bool>
+  -> {t' & Typed <`cons `nil {const 0} `Bool> 0 Bool t'}.
+  refine (
+      match prog with
+      | ty_lambda t' => fun _ _ _ => (existT _ _ (cast t'))
+      | _ => _ (* This catchall creates cases for all the other constructors *)
+      end
+    );try solve[intros; solve_all].
+Defined.
+
+(* I don't think that I can directly make a match with a notation *)
+(*Notation "'fancymatch' prog 'with' cases" := (match 10 with cases end) (at level 100).*)
+
+Axiom uip : forall T (t1 t2 : T) (p1 p2 : t1 = t2), p1 = p2.
+Theorem remove_cast
+        (ctx ty tm : QTerm)
+        (lvl : nat)
+        (pctx : ctx = ctx)
+        (plvl : lvl = lvl)
+        (pty : ty = ty)
+        (ptm : tm = tm)
+        (input : Typed ctx lvl ty tm)
+        : @cast _ _ _ _ _ _ _ _ pctx plvl pty ptm input = input.
+Proof.
+  rewrite (uip _ _ _ pctx eq_refl).
+  rewrite (uip _ _ _ plvl eq_refl).
+  rewrite (uip _ _ _ pty eq_refl).
+  rewrite (uip _ _ _ ptm eq_refl).
+  reflexivity.
+Qed.
+
+Ltac escape_transport_hell :=
+  repeat (rewrite (*?push_transport_through, ?compose_transport,*) ?remove_cast).
+
+Theorem match_on_id_works : match_on_id' (ty_lambda ty_true) eq_refl eq_refl eq_refl
+                            = existT _ _ ty_true.
+Proof.
+  simpl.
+  escape_transport_hell.
+  reflexivity.
+Qed.
+  
+Theorem push_transport_through
+        (P Q : QTerm -> nat -> QTerm -> QTerm -> Type)
+        (f : forall ctx lvl ty tm, P ctx lvl ty tm -> Q ctx lvl ty tm)
+        (ctx1 ctx2 ty1 ty2 tm1 tm2 : QTerm)
+        (lvl1 lvl2 : nat)
+        (pctx : ctx1 = ctx2)
+        (plvl : lvl1 = lvl2)
+        (pty : ty1 = ty2)
+        (ptm : tm1 = tm2)
+        (input : Typed ctx1 lvl1 ty1 tm1)
+  : f _ _ _ _ (@cast _ _ _ _ _ _ _ _ pctx plvl pty ptm input)
+    = @cast _ _ _ _ _ _ _ _  pctx plvl pty ptm (f _ _ _ _ input).
+Proof.
+  refine (match p with
+          | eq_refl => _
+          end).
+  reflexivity.
+Qed.
+
+Theorem compose_transport
+        (I : Type)
+        (P : I -> Type)
+        (i1 i2 i3 : I)
+        (p : i1 = i2)
+        (q : i2 = i3)
+        (input : P i1)
+  : transport P q (transport P p input) = transport P (eq_trans p q) input.
+Proof.
+  subst.
+  reflexivity.
+Qed.
+
