theories/metaprogramming/testRewriteIssue.v
@@ -1,0 +1,77 @@
+Require Import String.
+Require Import qterm.
+Require Import lambdaFacts.
+Require Import lambdaSolve.
+Require Import FunctionalExtensionality.
+Require Import Coq.Logic.PropExtensionality.
+
+Theorem thm : 1 = 1.
+Proof.
+  reflexivity.
+Qed.
+
+Theorem evarExample : True.
+Proof.
+  evar (x : nat).
+  assert (x = x). {
+    subst x.
+    Fail rewrite thm.
+    (* It doesn't look like rewrites just rewrite existentials arbitrarily *)
+    reflexivity.
+  }
+  constructor.
+  Unshelve.
+  apply 20.
+Qed.
+
+Theorem testThing (t1 t2 : QTerm) : lift "name" 0 t1 = t2.
+Proof.
+  evar (et1 : QTerm).
+  assert (et1 = t1) by give_up.
+  rewrite <- H.
+  unfold et1.
+  rewrite lift_lam.
+  (* So for some reason the rewrite does (incorrectly) work here, specializing the evar.
+   It doesn't work if the lhs is JUST an evar. Maybe part of the pattern has to exist? *)
+Abort.
+
+Theorem equality : 1 + 1 = 2. Proof. reflexivity. Qed.
+
+Theorem testRewrite2 (x : nat) : 1 + x = 2.
+  evar (ex : nat).
+  assert (ex = x).
+  2: {
+    rewrite <- H.
+    unfold ex.
+    (* The goal is now: "1 + ?ex = 2"
+       The rewrite tactic below specializes ?ex to 1 *)
+    rewrite equality.
+    reflexivity.
+  }
+Abort.
+
+Ltac hide_evar :=
+  repeat match goal with
+  | [ |- context [ ?v ] ] => is_evar v; let H := fresh v in pose (H := v); fold H
+  end.
+
+Theorem testRewrite2 (x y z : nat) : (1 + x) + (1 + x) + (1 + y) + (1 + y) = 2.
+  assert ((1 + x) + (1 + y) + (1 + y) + (1 + z) + (1 + z) = 2) as H by give_up.
+  evar (ex : nat).
+  assert (ex = x) by give_up.
+  rewrite <- H0 in *.
+  evar (ey : nat).
+  assert (y = ey) by give_up.
+  rewrite H1 in *.
+  evar (ez : nat).
+  assert (z = ez) by give_up.
+  rewrite H2 in *.
+  unfold ex, ey, ez in *.
+
+  let H := fresh v in pose (H := ?ex).
+  fold v in *.
+  
+  hide_evar.
+  rewrite equality.
+Abort.
+  
